\documentclass{article}
\usepackage[utf8]{inputenc} % Required for inputting international characters
\usepackage[T1]{fontenc} % Output font encoding for international characters

\input{preamble}
\input{macros}

\graphicspath{{./images/}}

\title{\huge{AEA June '02}}
\author{\huge{Jack Maguire}}
\date{}

\begin{document}
\maketitle

\qs{
	\begin{align*}
		&= \sin 5x \\
		&= \sin 2x \cos 3x + \sin 3x \cos 2x \\
		&= 2 \sin x \cos x \cos 3x + \sin 3x \left( \cos^2 x - \sin^2 x \right) \\
		&= 2 \sin x \cos x \left( \cos x \cos 2x - \sin x \sin 2x \right) + \left( \sin 2x \cos x + \sin x \cos 2x \right) \left( \cos^2 x - \sin^2 x \right) \\
		&= 2 \sin x \cos x \left( \cos x \left( \cos^2 x - \sin^2 x \right) - 2 \sin^2 x \cos x  \right) + \left( 2\sin x \cos^2 x + \sin x \left( \cos^2 x - \sin^2 x \right) \right) \left( \cos^2 x - \sin^2 x \right) \\
		&= 2 \sin x \cos x \left( \cos^3 x - \sin^2 x \cos x - 2 \sin^2 x \cos x \right) + \left( 2\sin \cos^2 x  + \sin x \cos^2 x - \sin^3 x\right) \left( \cos^2x - \sin^2x \right) \\
		&= 2 \sin x \cos x \left( \cos^3 x - 3\sin^2 x \cos x \right) + \left( 3\sin x \cos^2 x - \sin^3 x\right) \left( \cos^2x - \sin^2x \right) \\
		&= 2 \sin x \cos^4 x - 6 \sin^3 x \cos^2 x + 3\sin x \cos^4 x - \sin^3 x \cos^2 x - 3\sin^3 \cos^2 x + \sin^5 x \\
		&= 5 \sin x \cos^4 x - 10 \sin^3 x \cos^2 x + \sin^5 x \\
		\\
		&= \cos 5x \\
		&= \cos 3x \cos 2x - \sin 3x \sin 2x \\
		&= \left( \cos 2x \cos x - \sin 2x \sin x \right) \left( \cos^2 x - \sin^2 x \right) - 2 \sin x \cos x \left( \sin 2x \cos x + \sin x \cos 2x \right) \\
		&= \left( \left( \cos^2x - \sin^2x \right) \cos x - 2 \sin^2 x \cos x\right) \left(\cos^{2}x-\sin^{2}x\right) - 2 \sin x \cos x \left( 2 \sin x \cos^2 x + \left( \cos^2x - \sin^2x \right) \sin x \right) \\
		&= \left( \cos^3 x - \sin^2 x \cos x - 2 \sin^2 x \cos x \right) \left( \cos^2 x - \sin^2 x \right) - 2 \sin x \cos x \left( 2 \sin x \cos^2 x + \cos^2x \sin x - \sin^3 x \right) \\
		&= \left( \cos^3 x - 3 \sin^2 x \cos x \right) \left( \cos^2 x - \sin^2 x  \right) - 2 \sin x \cos x \left( 3 \sin x \cos ^2 x - \sin ^3 x \right) \\
		&= \cos^5 x - \sin^2 x \cos ^3 x - 3 \sin^2 x \cos^3 x + 3 \sin^4 x \cos x - 6 \sin^2 x \cos^3 x + 2 \sin^4 x \cos x \\
		&= \cos^5 x - 10 \sin^2 x \cos^3 x + 5 \sin^4 x \cos x \\
	\end{align*}
	\begin{align*}
		\sin x - \cos x &= \sin 5x - \cos 5x \\
		\sin x - \cos x &= 5 \sin x \cos^4 x - 10 \sin^3 x \cos^2 x + \sin^5 x - \cos^5 x + 10 \sin^2 x \cos^3 x - 5 \sin^4 x \cos x
		\textbf{???}
	\end{align*}
}
\qs{
	\begin{align*}
		\acb{p}{2} (1)^{p-2} (-4)^2 &= \acb{p}{4} (1)^{p-4} (-4)^4 \\
		4p(p-1) &= \frac{32p(p-1)(p-2)(p-3)}{3} \\
		3p(p-1) &= 8p(p-1)(p-2)(p-3) \\
		3 &= (p-2)(p-3) \\
		3 &= p^2 - 5p + 6 \\
		0 &= p^2 - 5p + 3 \\
		p &= \frac{5 \pm \sqrt{13}}{2} \\
		\\
		\acb{p}{3} (1)^{p-3} (-4)^3 &\geq 0 \\
		\frac{32p(p-1)(p-2)}{3} &\leq 0 \\
		\frac{32 * \frac{5 + \sqrt{13}}{2} * (\frac{5 + \sqrt{13}}{2} - 1)}{3} &= 0	\\
		\frac{32 * \frac{5 - \sqrt{13}}{2} * (\frac{5 - \sqrt{13}}{2} - 1)}{3} &= 0	\\
		p &= \frac{5 \pm \sqrt{13}}{2} 
	\end{align*}
}
\qs{
	\[ \differen = \frac{\Delta y \div \Delta t}{\Delta x \div \Delta t}=\frac{y^\prime(t)}{x^\prime(t)} \]
	\begin{multicols}{2}
		\noindent
		\begin{align*}
			x &= 15t-t^3 \\
			x^\prime &= 15-3t^2
		\end{align*}
		\columnbreak
		\begin{align*}
			y &= 3-2t^2 \\
			y^\prime &= -4t \\
		\end{align*}
	\end{multicols}

	\[ \differen = \frac{-4t}{15-3t^2} \]
	
	\begin{multicols}{2}
		\noindent
		\begin{align*}
			x &= 15t-t^3 \\
			14 &= 15t-t^3 \\
			0 &= -t^3 + 15t - 14 \\
			t &= 1, \ldots
		\end{align*}
		\columnbreak
		\begin{align*}
			y &= 3-2t^2 \\
			1 &= 3-2t^2 \\
			0 &= -2t^2 + 3t - 1 \\
			t &= 1, 0.5
		\end{align*}
	\end{multicols}

	\begin{align*}
		t &= 1 \\
		\differen_1 &= \frac{-4}{15-3} \\
		&= - \frac{1}{3} \\
		\therefore & \text{Normal} = 3 \\ \\
		3 &= \frac{-4t}{15-3t^2} \\
		45 - 9t^2 &= -4t \\
		0 &= 9t^2 - 4t - 45 \\
		t &= \frac{2 \pm \sqrt{409}}{9}
	\end{align*}
}
\qs{
	\begin{align*}
		x^3 + y^3 - 3xy &= 48 \\
		y^3 -3xy &= 48 - x^3 \\
		y \left( y^2 - 3x \right) &= 48 - x^3
		\textbf{???}
	\end{align*}
}

\qs{
\qsp{a}{
	\[ y = \sin \left( \cos x \right) \]
	\begin{multicols}{2}
		\noindent
		\begin{align*}
			0 &= \sin \left( \cos x \right) \\
			0 &= \cos x \\
			x &= \pm \frac{\pi}{2}
		\end{align*}
		\columnbreak
		\begin{align*}
			y &= \sin \left( \cos 0 \right) \\
			y &= \sin 1 \\
			y &= 0.841 
		\end{align*}
	\end{multicols}

	\begin{tabular}{rl}
		A & \( (- \frac{\pi}{2}, 0) \) \\
		B & \( (\frac{\pi}{2}, 0) \) \\
		C & \( (0, 0.841) \)
	\end{tabular}
}
\qsp{b}{
	\begin{align*}
		y &= \sin \left( \cos x \right) \\
		u &= \cos x \\
		\frac{\Delta x}{\Delta u} &= \sin x \\
		\differen &= - \cos \left( \cos x \right) \sin x \\
		\differen_0 &= 0
	\end{align*}
	\( \differen_0 = 0 \therefore B\) is a stationary point. 
}
\qsp{c, d}{
	\textbf{I know how to show this using a graph, but I'm not sure how to do this using algebra.}
}
}

\qs{
\qsp{a}{
	\begin{align*}
		m_2 - x^{n_2} &= m_1 - x^{n_1} \\
		m_2 - x^{12 - n_1} &= m_1 - x^{n_1} \\
	\end{align*}
	\begin{multicols}{2}
		\noindent
		\begin{align*}
			x &= 3 \\
			m_2 - 3^{12 - n_1} &= m_1 - 3^{n_1}  \\
			m_2 - \frac{3^{12}}{3^{n_1}} &= m_1 - 3^{n_1}
		\end{align*}
		\columnbreak
		\begin{align*}
			x &= -3 \\
			m_2 - (-3)^{12 - n_1} &= m_1 - (-3)^{n_1}  \\
			m_2 - \frac{-3^{12}}{-3^{n_1}} &= m_1 - (-3)^{n_1} \\
			m_2 - \frac{3^12}{3^{n_1}} &= m_1 - (-3)^{n_1}
		\end{align*}
	\end{multicols}
	\textbf{???}
}
}

\qs{
\qsp{a}{
	You can only separate brackets if you fully factorise, with factors on one side and a zero on the other - you separate brackets by dividing by each set of brackets. This only works with zero - because \( \frac{0}{x} \equiv 0 \).
}
\qsp{b}{
	\begin{align*}
		x^3 + \frac{3}{4}x - \frac{1}{2} &= 0 \\
		\func{\frac{1}{2}} &= 0 \\
		(x - \frac{1}{2})(x^2 + bx + 1) &= 0 \\
		\ldots - \frac{1}{2}x^2 + bx^2 + \ldots &= 0 \\
		-\frac{1}{2} + b &= 0 \\
		b &= \frac{1}{2} \\
		x^3 + \frac{3}{4}x - \frac{1}{2} &\equiv (x - \frac{1}{2})(x^2 +\frac{1}{2}x + 1) \\ \\
		x^2 +\frac{1}{2}x + 1 &= 0
		\Delta &= b^2 - 4ac \\
		&= \frac{1}{2}^2 - 4*1*1 \\
		&= - \frac{15}{4}
	\end{align*}
	\(\Delta < 0 \therefore\) no real solutions.
}
\qsp{c, d}{
	\textbf{???}
}
}
	
\end{document}