\documentclass{article}
\usepackage[utf8]{inputenc} % Required for inputting international characters
\usepackage[T1]{fontenc} % Output font encoding for international characters

\input{preamble}
\input{macros}

\graphicspath{{./images/}}

\title{\huge{C3 X}}
\author{\huge{Jack Maguire}}
\date{}

\begin{document}

\maketitle


\qs{
\qsp{a}{
	\[ y = \frac{x^2 - 6x + 12}{4x - 11} \]
	\begin{multicols}{2}
		\noindent
		\begin{align*}
			v &= 4x - 11 \\
			v^\prime &= 4 
		\end{align*}
		\pagebreak
		\begin{align*}
			u &= x^2 - 6x + 12 \\
			u^\prime &= 2x - 6
		\end{align*}
	\end{multicols}
	\noindent
	\begin{align*}
		\differen &= \frac{vu^\prime - v^\prime u}{v^2} \\
				  &= \frac{(4x-11)(2x-6) - 4(x^2-6x+12)}{(4x-11)^2} \\
				  &= \frac{8x^2 -46x + 66 - 4x^2 + 24x - 48}{(4x-11)^2} \\
				  &= \frac{4x^2 -22x + 18}{(4x-11)^2} \\
				  &= \frac{4x^2 -22x + 18}{16x^2 - 88x + 121} \\
	\end{align*}
}
\qsp{b}{
	\(y\) is decreasing \(\therefore \differen < 0\)
	
	\[ \frac{4x^2 -22x + 18}{16x^2 - 88x + 121} < 0 \]
	Since \( 16x^2 - 88x + 121 \) only has one repeated root, and is a positive curve, it will never go below zero, so we can ignore solutions from it.
	
	\begin{align*}
		 \frac{4x^2 -22x + 18}{16x^2 - 88x + 121} &< 0 \\
		 4x^2 -22x + 18 &< 0 \\
		 (2x-1)(4x-9) &< 0 \\
		 1 < x < 4.5 &
	\end{align*}
}
}

\qs{
\begin{align*}
	\sin 2\theta &= \cot \theta \\
	2\sin \theta \cos \theta &= \frac{\cos \theta}{\sin \theta} \\
	2\sin ^2 \theta \cos \theta &= \cos \theta \\
	2\sin ^2 \theta \cos \theta - \cos \theta &= 0\\
	\left( \cos \theta \right) \left(  2\sin ^2 \theta - 1  \right) &= 0
\end{align*}
\begin{multicols}{2}
	\noindent
	\begin{align*}
		\cos \theta &= 0 \\
		\theta &= 90 \dg
	\end{align*}
	\columnbreak
	\begin{align*}
		 2\sin ^2 \theta - 1 &= 0 \\
		 \sin ^2 \theta &= \frac{1}{2} \\
		 \sin \theta &= \pm \frac{\sqrt{2}}{2} \\
		 \theta &= 45 \dg, 135 \dg
	\end{align*}
\end{multicols}
\[ \theta = 45 \dg, 90 \dg, 135 \dg \]
}

\qs{
\qsp{a}{
	\begin{align*}
		&= \func{1 + \sqrt{9}} \\
		&= \func{4} \\
		&= 1 + \sqrt{4} \\
		&= 3
	\end{align*}
}
\qsp{b}{
	\begin{align*}
		y &= 1 + \sqrt{x} \\
		x &= 1 + \sqrt{y} \\
		x - 1 &= \sqrt{y} \\
		(x-1)^2 &= y \\
		\func{x} &= (x-1)^2
	\end{align*}
}
\qsp{c}{
	\includegraphics[width=\textwidth / 3]{x3c}
}
\qsp{d}{
	\begin{align*}
		1 + \sqrt{x} &= (x-1)^2 \\
		\sqrt{x} &= x^2 - 2x \\
		x &= \left( x^2 - 2x \right) ^2 \\
		0 &= x^4 - 4x^3 + 4x^2 - x
	\end{align*}
	We could say that \(x = 0\), but we can see it is invalid on the graph and ignore it.
	\begin{align*}
		\func{x} &= x^3 - 4x^2 + 4x - 1 \\
		\func{1} &= 1 - 4 + 4 - 1 = 0 \\
		0 &= (x-1)(x^2 + bx + 1) \\ 
		0 &= \ldots - x^2 + bx^2 + \ldots \\
		-1 + b &= -4 \\
		b &= -3 \\
		\func{x} &= (x-1)(x^2-3x+1)
	\end{align*}
	We could say that \(x = 1\), but we can see it is invalid on the graph and ignore it.
	\begin{align*}
		0 &= x^2 - 3x + 1 \\
		x &= \frac{-b \pm \sqrt{b^2-4ac}}{2a} \\
		&= \frac{3 \pm \sqrt{9 - 4}}{2} \\
	\end{align*}
	We could say that \(x = \frac{3 - \sqrt{5}}{2}\), but we can see it is invalid on the graph and ignore it.
	\[ x = \frac{3 + \sqrt{5}}{2} \]
}
}

\qs{
\qsp{a}{
	\begin{align*}
		\frac{\Delta y}{\Delta x} &= \frac{3y^2 - 4}{y^3-4y} \\
		\differen &= \frac{y^3-4y}{3y^2-4} \\
		2 &= \frac{3y^2-4}{y^3-4y} \\
		1 &= \frac{3y^2-4}{2y^3-8y} \\
		2y^3-8y &= 3y^2-4
		y &= \frac{3y^2-4}{2y^2-8} \\
		???
	\end{align*}
}
\qsp{b}{
	???
}
}

\qs{
\begin{align*}
	\differen &= (-1) \left(4e^{2-x}\right)-(-2) \left(e^{4-2x}\right) \\
			  &= -4e^{2-x} + 2e^{4-2x} \\
	0 &= -4e^{2-x} + 2e^{4-2x} \\
	2e^{2-x} &= e^{4-2x} \\
	2e^{2-x} &= \left( e^{4-2x} \right) ^2 \\ \\
	\text{Let } y &= e^{2-x} \\
	2y &= y^2 \\
	0 &= y^2 - 2y \\
	y &= 0, 2 \\
	\ln{0} &\nequiv \bbR \\
	e^{2-x} &= 2 \\
	x &= 2 - \ln{2} \\
	&= 1.307 \\ \\
	y &= 4e^{2-x} - e^{4-2x} \\
	&= 4 \\ \\
	\differen_{1.25} &= 0.49 \\
	\differen_{1.307} &= 0 \\
	\differen_{1.35} &= -0.32 \\
\end{align*}
\begin{itemize}
	\ii Stationary Point = \((1.307, 4)\)
	\ii Kind = Maximum
\end{itemize}
}

\qs{
\qsp{a}{
	???
}
\qsp{b}{
	\begin{align*}
		R \cos \left( \theta - \alpha \right) &= R\cos \theta \cos \alpha + R\sin \theta \sin \alpha \\
		\\
		R \sin \alpha &= 2 \\
		R \cos \alpha &= 5 \\
		\tan \alpha &= \frac{2}{5} \\
		\alpha &= 21.8 \\
		\\
		R^2 &= 5^2 + 2^2 \\
		R &= \sqrt{25 + 4} \\
		R &= \sqrt{29} \\
		\\
		5\cos \theta + 2\sin \theta &\equiv \sqrt{29} \cos \left( \theta - 21.8 \dg \right)
	\end{align*}
}
\qsp{c}{
	???
}
}

\qs{
\qsp{a}{
\begin{enumerate}
	\ii Take the natural logarithm of x value.
	\ii Shift the graph right by 12 units.
	\ii Shrink the graph horizontally by a factor of 4.
\end{enumerate}
}
\qsp{b}{
	\includegraphics[width=\textwidth / 3]{x7b}
}
}

\qs{
\qsp{a}{
	\begin{multicols}{2}
		\noindent
		\begin{align*}
			v &= x \\
			v^\prime &= 1 \\
		\end{align*}
		\begin{align*}
			u &= \sqrt{x+1} \\
			u^\prime &= \frac{1}{2}(x+1)^{-\frac{1}{2}}
		\end{align*}
	\end{multicols}
	\begin{align*}
		\differen &= vu^\prime + v^\prime u \\
		&= x\frac{1}{2}(x+1)^{-\frac{1}{2}} + (x+1)^{\frac{1}{2}} \\
		&= (x+1)^{-\frac{1}{2}}\left( x\frac{1}{2} + (x+1) \right) \\
		&= (x+1)^{-\frac{1}{2}}\left( \frac{3}{2}x+1 \right) \\
		&= \frac{1}{2}(3x+2)(x+1)^{-\frac{1}{2}}
	\end{align*}
}
\qsp{b}{
	\begin{multicols}{2}
		\noindent
		\begin{align*}
			v &= x\sqrt{x+1} \\
			v^\prime &= \frac{1}{2}(3x+2)(x+1)^{-\frac{1}{2}}
		\end{align*}
		\columnbreak
		\begin{align*}
			u &= \sin 2x \\
			u^\prime &= 2\cos 2x
		\end{align*}
	\end{multicols}
	\begin{align*}
		\differen &= vu^\prime + v^\prime u \\
		&= \left( x\sqrt{x+1} \right) \left( 2\cos 2x \right) + \left( \frac{1}{2}(3x+2)(x+1)^{-\frac{1}{2}} \right) \left( \sin 2x \right) \\
		&= \left( \frac{\pi}{2}\sqrt{\frac{\pi}{2}+1} \right) \left( 2\cos \pi \right) + \left( \frac{1}{2}(3\frac{\pi}{2}+2)(\frac{\pi}{2}+1)^{-\frac{1}{2}} \right) \left( \sin \pi \right) \\
		&= -2 \left( \frac{\pi}{2}\sqrt{\frac{\pi}{2}+1} \right)
	\end{align*}
}
}

\end{document}
