\documentclass{article}
\usepackage[utf8]{inputenc} % Required for inputting international characters
\usepackage[T1]{fontenc} % Output font encoding for international characters

\input{preamble}
\input{macros}

\graphicspath{{./images/}}

\title{\huge{C3 Y}}
\author{\huge{Jack Maguire}}
\date{}

\begin{document}
	
\maketitle

\qs{
	\begin{multicols}{2}
		\begin{multicols}{2}
			\noindent
			\begin{align*}
				v &= e^{-x} \\
				v^\prime &= -e^{-x}
			\end{align*}
			\columnbreak
			\noindent
			\begin{align*}
				u &= \sin x \\
				u^\prime &= \cos x 
			\end{align*}
		\end{multicols}
	
		\begin{align*}
			\differen &= vu^\prime + v^\prime u \\
			&= e^{-x}\cos x + -e^{-x} \sin x \\
			0 &= e^{-x}\cos x -e^{-x} \sin x \\
			&= \left( e^{-x} \right) \left( \cos x - \sin x \right) \\
			\bbR &\nsubseteq e^{-x} \\	
			0 &= \cos x - \sin x \\
			\cos x &= \sin x \\
			\tan x &= 1 \\
			x &= \frac{1}{4}\pi
		\end{align*}
	
		\columnbreak
		\noindent
		
		\begin{align*}
			e^{-x} &= e^{-x} \sin x \\
			1 &= \sin x \\
			x &= \frac{1}{2}\pi 
		\end{align*}
	\end{multicols}
	\begin{align*}
		&= \frac{1}{2} \pi - \frac{1}{4} \pi \\
		&= \frac{1}{4} \pi
	\end{align*}
}

\qs{
\qsp{a}{
	\[ R \sin \left( x + \alpha \right) \equiv R \sin \alpha \cos x + R \sin \alpha \cos x \]
	\begin{multicols}{2}
		\noindent
		\begin{align*}
			R^2 &= 2^2 + 1^2 \\
			R &= \sqrt{5}
		\end{align*}
		\columnbreak
		\begin{align*}
			2 &= \sin \alpha \\
			1 &= \cos \alpha \\
			\tan \alpha &= 2 \\
			\alpha &= 1.107
		\end{align*}
	\end{multicols}
	\[ 2\cos x + \sin x \equiv \sqrt{5}\sin \left( x + 1.107 \right) \]
}
\qsp{b}{
	\[ - \sqrt{5} \le \func{x} \le \sqrt{5} \]
	\begin{align*}
		\func[g]{- \sqrt{5}} &= \frac{5}{5 + 5} = 2 \\
		\func[g]{0} &= \frac{5}{0 + 5} = 1 \\
		\func[g]{\sqrt{5}} &= \frac{5}{5 + 5} = 2 \\
	\end{align*}
	\[ 1 \le \func[g]{\func{x}} \le 2\]
}
}

\qs{
\qsp{a}{
	\begin{align*}
		10 &= Ae^{-k*0} \\
		A &= 10 \\ \\
		5 &= Ae^{-5k} \\
		5 &= 10e^{-5k} \\
		\frac{1}{2} &= e^{-5k} \\
		-5k &= \ln \frac{1}{2}  \\
		5k &= \ln 2 \\
		k &= \frac{1}{5} \ln 2
	\end{align*}
}
\qsp{b}{
	\begin{align*}
		M &= 10e^{-\frac{1}{5}t} \\
		\frac{\Delta M}{\Delta t} &= \left( -\frac{1}{5} \right) \left(10e^{-\frac{1}{5}t} \right) \\
		&= -2e^{-\frac{1}{5}t} \\
		\ln \left( \frac{1}{\sqrt{2}} \right) &= -2e^{-\frac{1}{5}t} \\
		\ln \sqrt{2} &= 2e^{-\frac{1}{5}t} \\
		\ln \sqrt[4]{2} &= e^{-\frac{1}{5}t} \\
		-\frac{1}{5}t &= \ln \left( \ln \sqrt[4]{2} \right) \\
		t &= -5 \ln \left( \ln \sqrt[4]{2} \right) \\
		t &= 8.764
	\end{align*}
}
}

\qs{
\qsp{a}{
	\begin{align*}
		&= \tan 2x \\
		&= \frac{\sin 2x}{\cos 2x} \\
	\end{align*}
	\begin{multicols}{2}
		\noindent
		\begin{align*}
			v &= \cos 2x \\
			v^\prime &= -2 \sin 2x
		\end{align*}
		\columnbreak
		\begin{align*}
			u &= \sin 2x \\
			u^\prime &= 2 \cos 2x \\
		\end{align*}
	\end{multicols}
	\begin{align*}
		\differen[] &= \frac{vu^\prime - v^\prime u}{v^2} \\
		&= \frac{2\cos^2 2x + 2\sin^2 2x}{\cos^2 2x} \\
		&= \frac{2}{\cos^2 2x} \\
		&= 2 \sec^2 2x
	\end{align*}
}
\qsp{b}{
	\begin{multicols}{2}
		\noindent
		\begin{align*}
			v &= 6x \\
			v^\prime &= 6 \\
		\end{align*}
		\columnbreak
		\begin{align*}
			u &= \tan 2x \\
			u^\prime &= 2 \sec^2 2x
		\end{align*}
	\end{multicols}
	\begin{align*}
		\differen &= vu^\prime + v^\prime u \\
		&= 12x \sec^2 2x + 6 \tan 2x \\
		\differen_{\frac{1}{8}\pi} &= \frac{12}{8}\pi \sec^2 \frac{1}{4}\pi + \tan \frac{1}{4}\pi \\
		&= 3\pi + 1 \\ \\
		y &= 6x \tan 2x \\
		&= \frac{6}{8}\pi \tan \frac{2}{8}\pi \\
		&= \frac{3}{4}\pi \\ \\
		y - y_1 &= m \left( x - x_1 \right)  \\
		y - \frac{3}{4}\pi &= (3\pi + 1)\left( x - \frac{1}{8}\pi \right) \\
		y &=  (3\pi + 1)x - \frac{3\pi + 1}{8}\pi + \frac{3}{4}\pi \\
		\therefore c &= - \frac{3\pi + 1}{8}\pi + \frac{3}{4}\pi \\
		&= \frac{6\pi}{8} - \frac{3\pi^2 + \pi}{8}  \\
		&= \frac{-3\pi^2 + 5\pi}{8} \\
		??? \textbf{Maybe } 3\pi + 6
	\end{align*}
}
}

\qs{
\qsp{a}{
	\begin{align*}
		0 &= \sqrt{1 - (2x-1)^2} \\
		&= 1 - \left( 4x^2 - 4x + 1 \right) \\
		&= -4x^2 + 4x \\
		&= x^2 - x \\
		&= x(x-1) \\
		x &= 0, 1 \\
		a &= 1 \\
	\end{align*}
}
\qsp{b}{
	\begin{align*}
		\func{a \div 2} &= \func{0.5} \\
		&= \sqrt{1 - (1 - 1)^2} \\
		&= \sqrt{1} \\
		&= 1 \\
		0 &\le \func{x} \le 1
	\end{align*}
}
\qsp{c}{
	\begin{enumerate}
		\ii Stretch graph horizontally by a factor of 2
		\ii Stretch graph vertically by a factor of 2
		\ii Shift graph downwards by 2 units
	\end{enumerate}
		\includegraphics[width=\textwidth / 3]{y5c}
}
\qsp{d}{
	Domain: \( 0 \le x \le 2 \) \qquad 
	Range: \( -2 \le \func{x} \le 0 \)
}
}

\qs{
\qsp{a}{
	\begin{align*}
		\frac{2\cot \theta}{1 + \cot^2 \theta} &\equiv \sin 2\theta \\
		\textbf{LHS} &\equiv \frac{2\cot \theta}{1 + \cot^2 \theta} \\
		&\equiv \frac{2 \cot \theta}{\csc^2 \theta} \\
		&\equiv 2 \frac{\cos \theta}{\sin \theta}  \sin ^2 \theta \\
		&\equiv 2 \cos \theta \sin \theta \equiv \sin 2 \theta \equiv	 \textbf{RHS} \qed
	\end{align*}
}
\qsp{b}{
	\begin{align*}
		4 \cot ^2 \theta + 1 &= 2 \sin 2 \theta \left( 1 + \cot^2 \theta \right) \\
		4 \left( \cot^2 \theta + 1 \right) - 3 &= \left( 4 \sin \theta \cos \theta \right) \left( \csc^2 \theta \right) \\
		4 \csc^2 \theta - 3 &= 4 \cot \theta \\
		\frac{4}{\sin^2 \theta} &= 4 \frac{\cos \theta}{\sin \theta} + 3  \\
		4 &= 4 \cos \theta \sin \theta + 3 \sin^2 \theta \\
		4 &= 2 \sin 2 \theta + 3 \sin^2 \theta \\
		0 &= 3 \sin^2 \theta + 2 \sin 2 \theta - 4 \\
		0 &= 3 \sin ^2 \theta + 4 \sin \theta \cos \theta - 4 \\
		\textbf{???} 
	\end{align*}
}
}
\qs{
\qsp{a}{
	\begin{multicols}{2}
		\noindent
		\begin{align*}
			y &= 3 \sin^{-1}(x-1) \\ \\
			y &=  3 \sin^{-1}(0-1) \\
			&= 3 * -\frac{1}{2} \pi \\
			&= -\frac{3 \pi}{2} \ans \\
			y &=  3 \sin^{-1}(2-1) \\
			&= 3 * \frac{1}{2} \pi \\
			&= \frac{3 \pi}{2} \ans \\ 
			\\
			0 &= 3 \sin^{-1}(x-1) \\
			\sin(0) &= 3x - 3 \\
			0 &= 3x - 3 \\
			3x &= 3 \\
			x &= 1
		\end{align*}
		\columnbreak
		\begin{align*}
			y &= 2 \cos^{-1}(x-1) \\ \\
			y &= 2 \cos^{-1}(0-1) \\
			&= 2 \pi \ans \\
			0 &= 2 \cos^{-1}(x-1) \\
			\cos(0) &= 2x - 2 \\
			1 &= 2x - 2 \\
			3 &= 2x \\
			x &= \frac{3}{2} \ans
		\end{align*}
	\end{multicols}
	\begin{align*}
		3 \sin^{-1}(x-1) &= 2 \cos^{-1}(x-1) \\
		3x - 3 &= \sin \left(2 \cos^{-1}(x-1)  \right) \\
		\textbf{???}
	\end{align*}
	\includegraphics[width=\textwidth / 3]{y7a}
}
\qsp{b}{
	\textbf{???}
}
}

\qs{
\qsp{a}{
	\begin{align*}
		\left| \func{x} \right| &= 12 \\
		k\left( x^2 - 4x \right) &= \pm 12 \\ 
		12 / 4 &= 3 \\
		k &= 3 \\ 
		\textbf{Clarification?} &
	\end{align*}
}
\qsp{b}{
	\begin{multicols}{2}
		\noindent
		\begin{align*}
			3 \left( x^2 - 4x \right) &= 12 \\
			x^2 - 4x - 4 &= 0 \\
			x &= 2 \pm 2 \sqrt{2}
		\end{align*}
		\columnbreak
		\begin{align*}
			-3 \left( x^2 - 4x \right) &= 12 \\
			x^2 - 4x + 4 &= 0 \\
			(x-2)^2 &= 0 \\
			x &= 2
		\end{align*}
	\end{multicols}
	\[ x = 2-2\sqrt{2} \quad 2 \quad 2+2\sqrt{2} \]
}
}

	
\end{document}